\documentclass[a4paper,11pt,english]{article}
\usepackage{.styles/basic}
\usepackage{.styles/envs}
\frenchspacing

\usepackage{circuitikz}

\usepackage{caption}
\usepackage{subcaption}

%%%%%%% Title %%%%%%%%%%%%%%%%%%%%%%%%%%%
\title{\textbf{Algebraic Topology} - Exercise Sheet 7}
\author{Tor Gjone (2503108) \& Michele Lorenzi (3461634)}

%%%%%%% Definitions %%%%%%%%%%%%%%%%%%%%%
\input{defs}

\newSimpleHeaderEnvironment{exercise}{Exercise }

\setlength{\parindent}{0cm}
\setlength{\parskip}{3pt}

\newcommand{\orth}{\bot}

\renewcommand{\S}[1]{\mathcal{S}(#1)}
%%%%%%%% Content %%%%%%%%%%%%%%%%%%%%%%%%
\begin{document}

\mmaketitle

\begin{exercise}[1]

Suppose $f_n \to f$ in the compact-open topology. That is for all $K \se
X$Â compact and for all $U \se Z$ open, such that $f(K)\se U$, there exists $N \in \N$, such that for all
$n \ge N$, $f_n(K) \se U$.

Let $x \in X$, then $\{x\} \se X$ is compact, so for all neighbourhoods $U$ of $f(x)$, there
exists $N\in\N$ such that, for all $n\ge N$, $f_n(x) \in U$. So $f_n \to
f$ pointwise (since $Z$ is Hausdorff, so that limits are unique).

Now let $X = Z = [0,1]$ and 
\[ f_n(x) = \pwf{
2nx &\tif x \le (2n)\i \\
2 - 2nx &\tif (2n)\i \le x \le n\i \\
0 &\tif n\i \le x
} \]

\begin{figure}[h]
\centering
\input{graph_fn_fig}
\caption{Graph of $f_n$.}
\label{fig:1}
\end{figure}

Then $f_n \to f = 0$ pointwise. However $f_n([0,1]) =
[0,1] \not\se [0,1/2)$, whereas $f([0,1]) = \{0\} \se [0,1/2)$. So $f_n$ does
not converge to $f$ in the compact-open topology.
\end{exercise}



\begin{exercise}[2]

It is easy to show that there are isomorphisms $\pi_{n}(F,e) \cong \pi_n(\Omega B,c_b)$. Indeed, since $p : E \to B$ is a Serre fibration, we have the long exact
sequence
\[ \cdots \to \pi_n(E,e) \to \pi_n(B,b) \to \pi_{n-1}(F,e) \to \pi_{n-1}(E,e) \to
\cdots \]
where $p\i(b)=e \in F$. Since $E$ is contractible we have $\pi_n(E,e) = 0$,
for $n \ge 0$. So the middle map is an isomorphism and thus 
\[ \pi_{n}(F,e) \cong \pi_{n+1}(B,b) \cong \pi_n(\Omega B,c_b) \]
for $n \ge 0$.

To show that $F$ and $\Omega B$ are homotopy equivalent we need to find a map $F\to\Omega B$ inducing these isomorphisms. A reasonable choice seems to be the map $f$ constructed using a deformation retraction $H$ of $E$ to the point $e$: for any point $x$ in the fiber,  $p\circ H(x,-)$ defines a loop at $b$. We need to show that this induces isomorphisms $\pi_n(F,x)\to\pi_n(\Omega B,f(x))$ for any $x\in F$ and any $n\geq0$, i.e. we are left to show injectivity and surjectivity of these maps. This can be done using the exponential law and the homotopy lifting property, but there is an easier proof: we can define a map $E\to B^{[0,1]}$ by considering $p\circ H(x,-)$ for any $x\in E$, then the long exact sequence for $F\to E\to B$ maps to the long exact sequence for $\Omega B\to B^{[0,1]}\to B$, and since $E$ and $B^{[0,1]}$ are contractible, by the five-lemma we obtain the claim.
\end{exercise}


\begin{exercise}[3](The solution to exercise 6.3 might be useful for reference.)

Given $\sigma \in \Sigma_3$, let $\Psi_\sigma$ be the composite map defined in
the exercise. 

Consider a pair $(\phi,\psi) \in \pi_1(X) \times \pi_1(X)$, with $\phi=[f]$ and $\psi=[g]$. The first isomorphism maps, this pair to the class $[(f,g)]$, which is mapped to $[h] \in \pi_0(E)$, where $h: \nb^2 \to E$ is such that $h |_{I_{0,1}} = f$ and $h |_{I_{1,2}} = g$. Furthermore $h|_{I_{0,2}}$ is homotopy equivalent to $fg$ (see figure). The map $\pi_0(\sigma^*)$ permutes these edges according to $\sigma$. The rest of the maps then restricts to the edges $I_{0,1}$ and $I_{1,2}$. 

\begin{figure}[h]
\centering
\input{triangle_fig_4}
\caption{}
\label{fig:my_label}
\end{figure}

Referring to the figure, it is quite clear that the action of swapping the vertices $0$ and $1$, reverses the orientation of $f$ and exchanges $g$ and $fg$. Then we see that:

\begin{eqnarray*}
\Psi_{(0\; 1)};&& (\phi, \psi) \mapsto (\phi^{-1}, \phi \psi) \\
\Psi_{(0\; 2)};&& (\phi, \psi) \mapsto (\psi^{-1}, \phi^{-1}) \\
\Psi_{(1\; 2)};&& (\phi, \psi) \mapsto (\phi\psi, \psi^{-1})
\end{eqnarray*}

Furthermore it is easy to observe that if $\sigma = \sigma_1 \sigma_2$, then $\Psi_\sigma = \Psi_{\sigma_1} \circ \Psi_{\sigma_2}$. So we are done since the tree other permutations are products of two of the cases listed above.
\end{exercise}

\end{document}
