\documentclass[a4paper,11pt,english]{article}
\usepackage{.styles/basic}
\usepackage{.styles/envs}
\frenchspacing

\usepackage{circuitikz}

\usepackage{caption}
\usepackage{subcaption}

%%%%%%% Title %%%%%%%%%%%%%%%%%%%%%%%%%%%
\title{\textbf{Algebraic Topology} - Exercise Sheet 8}
\author{Tor Gjone (2503108) \& Michele Lorenzi (3461634)}

%%%%%%% Definitions %%%%%%%%%%%%%%%%%%%%%
\input{defs}

\newSimpleHeaderEnvironment{exercise}{Exercise }

\setlength{\parindent}{0cm}
\setlength{\parskip}{3pt}

\usepackage{enumerate}

\DeclareMathOperator{\holim}{holim}

% I keep adding \ in from of the P's. This makes sure I get an error.
\def\P{\undefined}

%%%%%%%% Content %%%%%%%%%%%%%%%%%%%%%%%%
\begin{document}
\mmaketitle

\begin{exercise}[1]
\begin{enumerate}[(a)]
\item % a
Let $[\xi] \in \pi_m(\holim_n P_n)$. We have
\begin{equation}
\pi_m(q_k)([\xi]) = [q_k \circ \xi] \q\tand 
\Psi \circ \pi_m(q_{k+1}) ([\xi]) = (\omega_k)_\star [p_k \circ q_{k+1} \circ
\xi]
\end{equation}
where $q_k \circ \xi$ is a loop based at $\omega_k(0)$ and $p_k \circ q_{k+1}
\circ \xi$ a loop based at $\omega_k(1)$, both in $P_k$. 

By extending the second loop by $\omega_k$ (ie. applying $(\omega_k)_\star$)
both loops are based at $\omega_k(0)$.

We want to show that these two maps are base homotopic. 

Consider $\xi(-)_k : S^m \to P_k[0,k]$. We denote the adjoint map by 
$\hat \xi_k : S^m \times [0,1] \to P_k$. 
Then $\hat \xi_k$ defines an unbased homotopy from $q_k \circ \xi$ to $p_k \circ q_{k+1} \circ
\xi$. Indeed, for $x \in S^k$,
\begin{align*}
(q_k \xi)(x)_k &=& \xi(x)_k(0) = \hat \xi_k(x,0)& \q{\tand} \\
(p_k \circ q_{k+1} \circ \xi) (x) &=& p_k(\xi(x)_{k+1} (0)) = \xi(x)_k(1) = \hat
\xi_k(x,1)
\end{align*}

Furthermore 
\begin{equation}
\hat \xi_k (1,-) = \xi(1)_k = \omega_k. 
\label{eq:2}
\end{equation}

We define $H : S^m \times [0,1]$ 
\[ H(-,t) := (\omega_k|_[0,t])_\star (\hat \xi_k(-,t)). \]
\todo{add a figure}
Note that $H$ is continues by \pref{eq:2}. Then $H$ defines a based (at
$\omega_k(0)$) homotopy from $q_k \xi$ to $\omega_\star (p_k \circ q_{k+1}
\circ \xi)$. 

\item % b

Let $\xi = ([\xi_n])_{n\ge 0} \in \lim_n \pi_m(P_n, \omega_n(0))$, ie. $[\xi_n] \in
\pi_m(P_n, \omega_n(0))$ such that $\Psi_n([\xi_{n+1}]) = [\xi_n]$ for all $n\ge
0$. 

Let $H_n : S^m \times [0,1] \to P_n$ be a homotopy realizing $(\omega_n)_\star
(p_n \circ \xi_{n+1}) \sim \xi_n$  (based at $\omega_n(0)$).

Since the homotopy is based, it factors through the quotient $V = S^m \times [0,1] /
\left(\{x_0\} \times [0,1]\right)$ ($x_0\in \S^m$ denotes the base point). Let
$H_n': V \to P_n$ be the map defined by $H_n$. 

By the construction of the conjugation $(\omega_n)_\star$, we may defines a
homeomorphism $h_n : S^m \times [0,1] \to V$, such that $\wtil H_n = H_n' \circ
h_n$ defines a homotopy from $\xi_n$ to $p_n \circ \xi$ and $\wtil H_n(x_0,-) =
\omega_n$. Se figure \pref{fig:2} for a illustration of the construction in
dimension $m=1$.

\todo{add fig}

By the exponential adjunction $\til H_n$ defines a map $\bar H_n: S^m \to
P_n^{[0,1]}$. 

By the construction of $\bar H_n$, $\bar H_n(x_0) = \omega_n$ and $\bar H_{n+1}
(x)(1) = p( \xi_{n}(x) ) = p (\bar H_n(x)(0))$, so $\bar H = (\bar H_n)_{n \ge
0}$ represent an element in $\pi_m(\holim_n P_n,\omega)$.

Also $q_n (\bar H(x)) = \bar H_n(x)(0) = \xi_n (x)$ for all $x\in S^m$, so
$\pi_m(q_n)(\bar H) = \xi$.


\item % c

\end{enumerate}
\end{exercise}




\end{document}
