\sheet 3

\def \L{\mathbb{L}}
\def \O{\mathcal{O}}

\renewcommand{\Xi}{{\mbox{\larger[2]$\pmb\xi$}}}

\begin{document}
\mmaketitle

\begin{exercise}[1]\ 
\begin{enumerate}
\item[(i)]

\item[(ii)]
Let $V$ be an inner product space. Then $\O(0, V) = \Xi(0,V)_\infty \cong
V_\infty = S^V$,
since there is only one embedding of $0$ into $V$ and every element in $v$ is
orthogonal to $\{0\}$. So the two spectra are clearly objectives isomorphic and
the isomorphism is also clearly natural, so we get an isomorphism of orthogonal
spectra.
\end{enumerate}

\end{exercise}

\begin{exercise}[2]\ 
\begin{enumerate}
\item[(i)]
We need to check that 
\[ \lambda_\npi \circ (\sigma_n \wedge S^1) = (\sigma_\npi \wedge S^1) \circ
(S^1 \wedge \lambda_n). \]
Consider $v \wedge x \wedge w \in S^1 \wedge X_n \wedge S^1$, then
\begin{align*}
(\sigma_\npi \circ (\sigma^1 \wedge \lambda_n))(v \wedge x \wedge w) 
&= \sigma_\npi\Big(v \wedge \big\{ (n+1,...,2,1)\cdot\sigma_n(w \wedge x)\big\}\Big) \\
&= (n+2,...,3,2)\cdot\sigma_\npi(v \wedge \sigma_n(w\wedge x))) \\
&= (n+2,...,3,2) \cdot \sigma^2( (v \wedge w) \wedge x))) \\
&= (n+2,...,3,2) \cdot \sigma^2( (2,1) (w \wedge v) \wedge x))) \\
&= (n+2,...,3,2)(2,1) \cdot \sigma^2( (w \wedge v) \wedge x))) \\
&= (n+2,...,2,1) \cdot \sigma_\npi( w \wedge \sigma_n(v \wedge x)) \\
&= \lambda_\npi( \sigma_n(v \wedge x) \wedge w) \\
&= (\lambda_\npi \circ (\sigma_n \wedge S^1))(v \wedge x \wedge w).
\end{align*}

\item[(ii)]
\end{enumerate}
\end{exercise}

\begin{exercise}[3]\ 
Let $f : S^{n+k} \to X_n$ be a representative of an element in $\pi_k(X)$.
Since $\Sigma_m$ acts trivially on $X_m$ for infinitely many $m$, we may assume
wlog., that for $\Sigma_{n+2}$ acts trivially on $X_{n+2}$. 
% We have that 
So by $\Sigma_2 \times \Sigma_n$-equivariance of $\sigma^2$, the map
\[ \sigma^2 \circ (S^2 \smash f) : S^2 \smash S^n \to X_{2+n} \]
factors through the quotient space the action $\Sigma_2 \times
\Sigma_n$-action on. In particular it factors through the quotient space of the
$\Sigma_2$-action on $S^2$, which is isomorphic to $D^2$. However, $D^2$ is
contractible and the smash product with a contractible space is contractible.
So, in other words,
$\sigma^2 \circ (S^2 \smash f)$ factors through a contractible space, and thus 
$[f] = [\sigma_n \circ (S^2 \smash f)] = 0$.
\end{exercise}

\end{document}
