\sheet 2

\def \L{\mathbb{L}}
\def \simto{\xrightarrow{\sim}}
\def \O{\mathcal{O}}

\begin{document}
\mmaketitle

\begin{exercise}[1]\ 
\end{exercise}

\begin{exercise}[2]\ 
\begin{enumerate}
\item[(a)]
Fix a linear isometry $\psi: \R^n \simto W$. Let 
$q : X_n \to X^\flat(W)$ denote the quotient map 
\[ x \mapsto [\psi \wedge x]. \]
and define $\eta: X^\flat(W) \to X_n$ by 
\[ [\phi \wedge x] \mapsto (\psi^{-1} \circ \phi) . x. \]
Where $(\psi^{-1} \circ \phi)$ is consider as an element in $O(n)$ action on
$x$.

Then, for $x \in X^n$ and $\phi \in \L(\R^n, W)_+$ 
\begin{align*}
(q \circ \eta) ([x \wedge \phi]) 
&= [\psi \wedge (\psi^{-1} \circ \phi) . x ] 
= [\psi \circ \psi^{-1} \circ \phi \wedge x]
= [\phi \wedge x], \q{\tand} \\
(\eta \circ q) (x) 
&= (\psi^{-1} \circ \psi) . x 
= x
\end{align*}
Clearly both $q$ and $\eta$ are continues, proving the clime.

\item[(b)]
We denote the map in the exercise by $\mu$ and
let $A \in O(n)$, and $x, \psi, \phi$ as in the exercise, then 
\begin{align*}
\mu( \psi \wedge (\phi \circ A) \wedge x ) 
&= (\psi \circ \phi \circ A) \wedge x  \\
&\sim (\psi \circ \phi) \wedge A . x \\
&= \mu( \psi \wedge \phi \wedge A . x ) 
\end{align*}
So the map to descend ('factor' through) to the quotient. 

\item[(c)]
% We have the following diagram 
% \[ \begin{tikzcd}
% S^V \wedge \L(\R, W)_+ \wegde X_n \arrow[r]
% & \L(\R^{m+n}, V \oplus W)_+ \wedge X_{m+n} \\
% v \wedge \phi \wedge x \arrow[r, mapsto]
% & (\psi \oplus \phi) \wedge \sigma^m(\psi^{-1}(v)\wedge x)
% \end{tikzcd} \]

We have 
\begin{align*}
v \wedge (\phi \circ A) \wedge x 
&\mapsto (\psi \oplus (\phi \circ A)) \wedge \sigma^n(\psi^{-1}(v) \wedge x) \\
&\sim (\psi \oplus \phi) \wedge (I_m\oplus A) . \sigma^n (\psi^{-1}(v) \wedge x)
\\
&= (\psi \oplus \phi) \wedge \sigma^n (\psi^{-1}(v) \wedge A.x)
\end{align*}
Where $I_m \in O(m)$ is the unit matrix and $I_m\oplus A$ the diagonal block
matrix. So the mapping respects the equivalence relation. 

Let $\psi' : \R^m \to V$, then $\psi' = \psi \circ B$ for some $B \in O(m)$, and
we have
\begin{align*}
&(\psi' \oplus \phi) \wedge \sigma^n ((\psi')^{-1}(v) \wedge x) \\
&\sim (\psi \oplus \phi) \wedge (B \oplus I)\sigma^n ((\psi')^{-1}(v) \wedge x) \\
&= (\psi \oplus \phi) \wedge \sigma^n (\psi^{-1}(v) \wedge x) \\
\end{align*}
So the definition is independent of the choice of $\psi$.

\item[(d)]
To define an orthogonal spectra, we define a based continues functor $X^\flat :
\O \to T_*$. 


Let $U, V$ and $W$ denote inner product spaces, 
Firstly,we define $X^\flat (W)$ as in (a). Secondly we need to define 
$\mu_{V,W}: \O(V, W) \wedge X^\flat(V) \to X^\flat(W)$, satisfying
associativity, ie. 
\[ \begin{tikzcd}[column sep = 7em]
\O(V, W) \wedge \O(U,V) \wedge X^\flat(U) 
\arrow[r, "O(V{,}W) \wedge \mu_{U{,}V}"] 
\arrow[d, "\circ \wedge X^\flat(U)"] 
& \O(V, W) \wedge X^\flat(V) 
\arrow[d, "\mu_{V{,}W}"] \\ 
\O(U,W) \wedge X^\flat(U) 
\arrow[r, "\mu_{U{,}W}"] 
& X^\flat(W)
\end{tikzcd} \]
commutes. Furthermore, we want the functionality to be given as in (b) and the
structure maps as in (c), which may be expressed by the following to relations
\begin{equation}
\begin{split}
X^\flat(V,W) &= \mu_{V, W} \circ (j_{V,W} \wedge \id_{X^\flat(W)}) : 
\L(V, W)_+ \wedge X^\flat (V) \to X^\flat(W),
\\
\sigma_{V,W} &= \mu_{W,V\oplus W} \circ (i_V \wedge \id_{X^\flat(W)}) :
S^V \wedge X^\flat (W) \to X^\flat(V \oplus W).
\end{split}
\end{equation}
Where 
\begin{align*}
j_{V,W} : \L(U,W)_+ \into \O(V,W); & \phi \mapsto (0,\phi), \\
i_V : S^V \into \O(W, V\oplus W); & v \mapsto ((v,0), (0,\id_W)).
\end{align*}


We consider $(w, \xi) \in \Xi(V,W)$, $[\phi \wedge x] \in X^\flat(V)$. Let 
\[ W' = W/\im(\xi), \: m' = \dim(W') \q{\tand} \psi' : \R^{m'} \to W'. \]

Then we define $\mu$ as follows 
\[ \mu((w,\xi) \wedge [\phi \wedge \x]) :=
[ \psi \oplus (\xi \circ \phi) \wedge \sigma^m(\psi^{-1} \wedge x)] 
\]

This is clearly continues and extends continuously to $\O(V,W)$, since both
$\psi^{-1}$ and $\sigma^m$ extends continuously to the one point
compactification.

We check that this satisfy the associativity 
\begin{align*}

\end{align*}



\item[(e)]
\item[(f)]


\end{enumerate}
\end{exercise}

\end{document}
